Started adding the wrapping ocaml wrapper and parsing code.

checker/cOption.ml
@@ -1,0 +1,22 @@
+(* Option handling *)
+let infile = ref None
+let modules = ref []
+
+let verbosity = ref 0
+
+(* --------------------------------------------- *)
+(*       Specification list for options          *)
+(* --------------------------------------------- *)
+let (speclist:(Arg.key * Arg.spec * Arg.doc) list) =
+  Arg.align
+    [(
+      "-verbosity",
+      Arg.Set_int(verbosity),
+      "<int> : verbosity level, from 0 to 2 (default:0)"
+     ) ;
+     (
+       "-load",
+       Arg.String(fun m -> modules := m :: !modules),
+       "<string> : additional checker module to load."
+     );
+    ]
