checker/cOption.mli
@@ -1,0 +1,9 @@
+(** Options and command-line parsing **)
+val infile : string option ref
+val modules : string list ref
+val verbosity : int ref
+
+(* --------------------------------------------- *)
+(*       Specification list for options          *)
+(* --------------------------------------------- *)
+val speclist : (Arg.key * Arg.spec * Arg.doc) list ;;
