checker/checker.mli
@@ -1,0 +1,14 @@
+(* Type definitions for checkers. *)
+type checker = {
+  (* For logging purposes. *)
+  repr: string ;
+  
+  (* The actual check *)
+  check: MTypes.clause -> bool
+} 
+
+type t = checker
+
+(* Function for building a checker from
+ * a given type. *)
+type 'a builder = 'a -> t
