checker/mTypes.mli
@@ -1,0 +1,16 @@
+(* Types for models. *)
+type ident = string
+
+type ivar = int
+type bvar = int
+
+type vprop =
+| ILe of ivar*int
+| IEq of ivar*int
+| BTrue of bvar
+
+type lit =
+| Pos of vprop
+| Neg of vprop
+
+type clause = lit list
