checker/main.ml
@@ -1,0 +1,119 @@
+(* Top-level checker code. *)
+module List = ExtLib.List
+module L = List
+module GL = Genlex
+module MT = MTypes
+module C = Checker
+module M = Model
+module S = Spec
+
+module DL = Dynlink
+
+(* constraint(id) |- clause *)
+type inference = (MT.ident * MT.clause)
+
+let fmt = Format.std_formatter
+let err_fmt = Format.err_formatter
+
+let log_failure checker _ =
+  Format.fprintf fmt "Inference failed: %s |- {{FIXME}}."
+    (checker.C.repr) (* (MT.string_of_clause clause) *)
+
+let log info args =
+  Format.fprintf fmt info args ; Format.fprintf fmt "@."
+
+let check_inference model ident clause =
+  try
+    let checker = M.get_checker model ident in
+    let okay = checker.C.check clause in
+    if !COption.verbosity > 0 && not okay then
+      log_failure checker clause ;
+    okay
+  with Not_found ->
+    begin
+      log "Error: constraint not found: %s" ident ;
+      false
+    end
+
+let check_inferences model infs =
+  L.fold_left (fun b (id, cl) -> b && check_inference model id cl) true infs
+  
+let parse_defn spec = parser
+  | [< 'GL.Ident id ; 'GL.Kwd ":=" ; v = spec id >] -> v
+
+let term_defn model id =
+  let aux key = match key with
+  | "int" ->
+     begin parser
+       | [< >] -> M.add_ivar model id
+     end
+  | "bool" ->
+      begin parser
+        | [< >] -> M.add_bvar model id
+      end
+  | _ -> let pcon = Registry.find key in
+    begin parser
+      | [< 'GL.Kwd "(" ; checker = pcon ; 'GL.Kwd ")" >] ->
+          M.add_checker model id checker
+    end in
+  parser
+    | [< 'GL.Ident key ; v = aux key >] -> v
+
+let parse_clause model =
+  let parse_lit = parser
+    | [< 'GL.Kwd "~" ; 'GL.Ident id >] ->
+        MT.Neg (M.get_vprop model id)
+    | [< 'GL.Ident id >] ->
+        MT.Pos (M.get_vprop model id)
+  in S.listof parse_lit
+
+let parse_model =
+  let model = M.create () in
+  parser
+    | [< _ = S.listof (parse_defn (term_defn model)) >] -> model
+    (*
+  let aux = parser
+    | [< 'GL.Ident id ; 'GL.Kwd ":=" ; _ = (term_defn model id) >] -> ()
+    | [< >] -> ()
+  in parser
+    | [< 'GL.Kwd "[" ; _ = aux ; 'GL.Kwd "]" >] -> model
+    *)
+
+
+let parse_inferences model =
+  let parse_inf = parser
+    | [< 'GL.Ident id ; 'GL.Kwd "|-" ; cl = parse_clause model >] -> (id, cl)
+  in let rec aux = parser
+    | [< inf = parse_inf ; tail = aux >] -> inf :: tail
+    | [< >] -> []
+  in aux
+(*
+let parse_inferences = parser
+  | [< 'Ident id ; 'Kwd "|-" ; cl = (S.listof parse_lit) >] ->
+      (id, M.clause_of_model)
+*)
+
+let main () =
+  (* Parse the command-line arguments *)
+  Arg.parse
+    COption.speclist
+      (begin fun infile -> COption.infile := Some infile end)
+      "cp-certify <options> <inputfile>"
+  ;
+  (* Parse the program *)
+  let input = match !COption.infile with
+      | None -> stdin
+      | Some file -> open_in file
+  in
+  (* Register any additional checker modules. *)
+  List.iter (fun m -> DL.loadfile_private m) !COption.modules ;
+  let tokens = Spec.lexer (Stream.of_channel input) in 
+  let model = parse_model tokens in
+  let infs = parse_inferences model tokens in
+  let okay = check_inferences model infs in
+  if okay then
+    Format.fprintf fmt "OKAY@."
+  else
+    Format.fprintf fmt "FAILURE: invalid inference found.@." 
+
+let _ = main () 
