checker/model.ml
@@ -1,0 +1,75 @@
+(* Model specification. *)
+module MT = MTypes
+module H = Hashtbl
+module A = DynArray
+module C = Checker
+
+type ident = MT.ident
+
+(* Symbol kind. *)
+type ident_kind =
+| IdBool (* Bool variable *)
+| IdInt  (* Int variable *)
+| IdCon  (* Constraint (with associated checker) *)
+| IdProp (* Proposition *)
+
+type model = {
+  (* Symbol table. *)
+  symbols : (ident, ident_kind*int) Hashtbl.t;
+
+  bvar_names : ident A.t ;
+  ivar_names : ident A.t ;
+  constraints : (ident * C.t) A.t;
+  vprops : (ident * MT.vprop) A.t
+}
+
+type t = model
+
+let create () = {
+  symbols = Hashtbl.create 17 ;
+
+  bvar_names = A.create ();
+  ivar_names = A.create ();
+  constraints = A.create ();
+  vprops = A.create ();
+}
+
+(* Fixme: Add checking of duplicates. *)
+let add_ivar model ident =
+  let idx = A.length model.ivar_names in
+  Hashtbl.add model.symbols ident (IdInt, idx) ;
+  A.add model.ivar_names ident
+
+let add_bvar model ident =
+  let idx = A.length model.bvar_names in
+  Hashtbl.add model.symbols ident (IdBool, idx) ;
+  A.add model.bvar_names ident
+
+let add_vprop model ident prop =
+  let idx = A.length model.vprops in
+  Hashtbl.add model.symbols ident (IdProp, idx) ;
+  A.add model.vprops (ident, prop)
+
+let add_checker model ident checker =
+  let idx = A.length model.constraints in
+  Hashtbl.add model.symbols ident (IdCon, idx) ;
+  A.add model.constraints (ident, checker)
+
+let get_vprop (model : t) ident =
+  try
+    let (kind, idx) = Hashtbl.find model.symbols ident in
+    match kind with
+    | IdProp -> snd (A.get model.vprops idx)
+    | IdBool -> MT.BTrue idx
+    | _ -> failwith (Format.sprintf "Error: symbol %s not a proposition." ident)
+  with Not_found ->
+    failwith (Format.sprintf "Error: symbol not found - %s." ident)
+
+let get_checker model ident =
+  try
+    let (kind, idx) = Hashtbl.find model.symbols ident in
+    match kind with
+    | IdCon -> snd (A.get model.constraints idx)
+    | _ -> failwith (Format.sprintf "Error: symbol %s not a constraint." ident)
+  with Not_found ->
+    failwith (Format.sprintf "Error: symbol not found - %s." ident)
