checker/model.mli
@@ -1,0 +1,15 @@
+(* Types for models. *)
+type model
+
+type t = model
+
+val create : unit -> model
+
+val add_ivar : t -> MTypes.ident -> unit
+val add_bvar : t -> MTypes.ident -> unit
+val add_vprop : t -> MTypes.ident -> MTypes.vprop -> unit
+val add_checker : t -> MTypes.ident -> Checker.t -> unit
+
+val get_vprop : t -> MTypes.ident -> MTypes.vprop
+
+val get_checker : t -> MTypes.ident -> Checker.t
