checker/registry.ml
@@ -1,0 +1,16 @@
+(* Registry of checkers for constraint classes. *)
+module H = Hashtbl
+
+let registry = H.create 17
+
+(* Register a new checker kind. *)
+let add ident checker = H.add registry ident checker
+
+(* Find the checker-constructor for the given class. *)
+let find ident =
+  try
+    H.find registry ident
+  with
+    Not_found ->
+      failwith
+        (Format.sprintf "Checker not found for %s; using null checker." ident )
