checker/registry.mli
@@ -1,0 +1,7 @@
+(* Registry of checkers for constraint classes. *)
+
+(* Register a new checker kind. *)
+val add : MTypes.ident -> (Genlex.token Stream.t -> Checker.t) -> unit
+
+(* Find the checker-constructor for the given class. *)
+val find : MTypes.ident -> Genlex.token Stream.t -> Checker.t
