checker/spec.ml
@@ -1,0 +1,31 @@
+(* Parameter specifications for constraints. *)
+module S = Stream
+open Genlex
+
+type 'a spec = (token S.t -> 'a)
+
+let keywords = ["(";")";";";",";":=";"|-";"<=";"<";"~";"[";"]"]
+
+let lexer stream = 
+  let rec aux = parser
+    | [< 'h; t=aux >] -> [< 'h; t >]
+    | [< >] -> [< >] in
+    aux (make_lexer keywords stream)
+
+let ident = parser
+  | [< 'Ident s >] -> s
+let intconst = parser
+  | [< 'Int n >] -> n
+let boolconst = parser
+  | [< 'Ident s >] -> bool_of_string s
+
+let listof sub_parse =
+  let rec aux = parser
+    | [< k = sub_parse ; 'Kwd "," ; t = aux >] -> k :: t
+    | [< k = sub_parse >] -> [k]
+    | [< >] -> []
+  in parser
+    | [< 'Kwd "[" ; elts = aux ; 'Kwd "]" >] -> elts
+
+let cons p1 p2 = parser
+  | [< e1 = p1 ; e2 = p2 >] -> (e1, e2)
