checker/spec.mli
@@ -1,0 +1,10 @@
+(* Parameter specifications for constraints. *)
+val lexer : char Stream.t -> Genlex.token Stream.t
+
+type 'a spec = (Genlex.token Stream.t -> 'a)
+
+val ident : string spec
+val intconst : int spec
+val boolconst : bool spec
+val listof : 'a spec -> ('a list) spec
+val cons : 'a spec -> 'b spec -> ('a * 'b) spec
