checker/cumulative.v
@@ -2,12 +2,16 @@ Require Import ZArith.
 Require Import Bool.
 Require Import bounds.
 Require Import prim.
+Require Import Program.
+Require Import Program.Wf.
+
+Local Open Scope nat_scope.
 
 (* Really should add some stuff regarding
  * non-negative variables. *)
 Record task : Type := mkTask {
-  duration : Z ;
-  resource : Z ;
+  duration : nat ;
+  resource : nat ;
   svar : ivar 
 }.
 
@@ -19,27 +23,194 @@ Record vartask : Type := mkVarTask {
 
 Record cumul : Type := mkCumul {
   tasks : list task ;
-  limit : Z
+  limit : nat
 }.
 
-Fixpoint eval_usage (ts : list task) (time : Z) (theta : asg) :=
+Definition eval_start (t : task) (theta : asg) :=
+  eval_ivar t.(svar) theta.
+Definition eval_end (t : task) (theta : asg) :=
+  Zplus (eval_ivar t.(svar) theta) (Z_of_nat t.(duration)).
+
+Definition task_at_time (t : task) (time : nat) (theta : asg) : nat :=
+  let tstart := eval_start t theta in
+  let tend := eval_end t theta in
+  let ztime := Z_of_nat time in
+  if Z_leb tstart ztime && Z_ltb ztime tend then
+    t.(resource)
+  else
+    0%nat.
+
+Fixpoint eval_usage (ts : list task) (time : nat) (theta : asg) : nat :=
   match ts with
-  | nil => 0%Z
+  | nil => 0%nat
   | cons t ts' =>
-      let tstart := eval_ivar t.(svar) theta in
-      let curr :=
-        if Z_leb tstart time && Z_ltb time (tstart + t.(duration)) then
-          t.(resource)
-        else 0 in
-      curr + eval_usage ts' time theta
+      plus (task_at_time t time theta) (eval_usage ts' time theta)
   end.
 
 Definition eval_cumul (c : cumul) (theta : asg) :=
-  forall (time : Z), eval_usage c.(tasks) time theta <= c.(limit).
+  forall (time : nat), le (eval_usage c.(tasks) time theta) c.(limit).
+
+Fixpoint span_usage (ts : list task) (start : nat) (sz : nat) (theta : asg) :=
+  match sz with
+  | O => 0%nat
+  | S sz' =>
+     plus (eval_usage ts (start+sz-1) theta) (span_usage ts start sz' theta)
+  end.
+
+Theorem  span_usage_lim :
+  forall (c : cumul) (start : nat) (sz : nat) (theta : asg),
+    eval_cumul c theta ->
+      le (span_usage c.(tasks) start sz theta) (c.(limit) * sz).
+Proof.
+  unfold eval_cumul; intros.
+  induction sz.
+    unfold span_usage. omega.
+
+    unfold span_usage; fold span_usage.
+    assert (le (eval_usage (tasks c) (start + (S sz) - 1) theta) c.(limit)).
+    apply H.
+    rewrite <- mult_n_Sm.
+    rewrite plus_comm.
+    apply plus_le_compat.
+    apply IHsz.
+    exact H0.
+Qed.
+
+Theorem span_usage_split : forall (t : task) (ts : list task) (start sz : nat) (theta : asg),
+  span_usage (cons t ts) start sz theta =
+    plus (span_usage (cons t nil) start sz theta) (span_usage ts start sz theta).
+Proof.
+  intros. induction sz.
+    unfold span_usage; omega.
+
+    unfold span_usage ; fold span_usage.
+    assert (forall (i j k l : nat), plus (plus (plus i k)  j) l = (plus (plus i j)  (plus k l))).
+      intros. omega.
+    rewrite <- H.
+    unfold eval_usage at 1; fold eval_usage. unfold eval_usage at 2.
+    rewrite IHsz. omega.
+Qed.
+    
+Fixpoint task_usage (t : task) (start : nat) (sz : nat) (theta : asg) :=
+  match sz with
+  | O => 0%nat
+  | S sz' =>
+    plus (task_at_time t (start+sz-1) theta) (task_usage t start sz' theta)
+  end.
+Theorem task_usage_eq_span : forall (t : task) (start sz : nat) (theta : asg),
+  task_usage t start sz theta = span_usage (cons t nil) start sz theta.
+Proof.
+  intros; induction sz.
+    unfold task_usage, span_usage; trivial.
+
+    unfold task_usage, span_usage. fold task_usage; fold span_usage.
+    rewrite <- IHsz. unfold eval_usage. omega.
+Qed.
+Theorem task_in_span : forall (t : task) (time : nat) (theta : asg),
+  Zle (eval_start t theta) (Z_of_nat time)
+    /\ Zlt (Z_of_nat time) (eval_end t theta) ->
+      task_at_time t time theta = t.(resource).
+Proof.
+  intros; destruct H as [Hs He].
+  unfold task_at_time.
+  assert (Z_leb (eval_start t theta) (Z_of_nat time)
+    && Z_ltb (Z_of_nat time) (eval_end t theta) = true) as Ht.
+    apply andb_true_iff; rewrite Z_leb_iff_le; rewrite Z_ltb_iff_lt.
+    omega.
+  destruct andb.
+    trivial.
+    discriminate.
+Qed.
+Theorem task_usage_monotone_r : forall (t : task) (start sz sz' : nat) (theta : asg),
+  le sz sz' -> le (task_usage t start sz theta) (task_usage t start sz' theta).
+Proof.
+  intros.
+  induction sz'.
+    assert (sz = 0%nat) as Hsz0. omega.
+    rewrite Hsz0; trivial.
+    
+    assert (sz = (S sz') \/ sz < S sz'). omega.
+    destruct H0 as [Heq | Hlt].
+      rewrite Heq. omega.
+
+      unfold task_usage at 2;  fold task_usage.
+      assert (le O (task_at_time t (start + S sz' - 1) theta)). omega.
+      assert (forall (i j k : nat), i <= k -> i <= j + k). intros; omega. 
+      apply H1. apply IHsz'. apply lt_n_Sm_le. exact Hlt.
+Qed.
+(*
+Theorem task_duration_usage : forall (t : task) (start sz : nat) (theta : asg),
+  (Z_ge (Z_of_nat start) (eval_ivar t.(svar) theta) /\
+    (Z_of_nat (start + sz)) = (Zplus (eval_ivar t.(svar) theta) (Z_of_nat t.(duration)))) ->
+      task_usage t start sz theta = sz*t.(resource).
+Proof.
+  intros; induction sz.
+    unfold task_usage; trivial.
+
+    unfold task_usage; fold task_usage.
+*)
+
+Fixpoint span_usage_transp (ts : list task) (start : nat) (sz : nat) (theta : asg) :=
+  match ts with
+  | nil => 0%nat
+  | cons t ts' => plus (task_usage t start sz theta) (span_usage_transp ts' start sz theta)
+  end.
+
+Theorem span_usage_eq_transp : forall (ts : list task) (start sz : nat) (theta : asg),
+  span_usage ts start sz theta = span_usage_transp ts start sz theta.
+Proof.
+  intros; induction ts.
+    induction sz.
+        unfold span_usage, span_usage_transp; trivial.
+
+        unfold span_usage; fold span_usage.
+        rewrite IHsz.
+        unfold span_usage_transp.
+        unfold eval_usage. omega.
+
+    unfold span_usage_transp; fold span_usage_transp.
+    rewrite <- IHts.
+    rewrite span_usage_split.
+    rewrite <- task_usage_eq_span.
+    trivial.
+Qed.
+
+Definition task_bracketed (t : task) (start sz : nat) (theta : asg) :=
+  Zle (Z_of_nat start) (eval_ivar t.(svar) theta)
+    /\ Zlt (eval_end t theta) (Z_of_nat (start + sz)).
+
+(*
+Theorem task_cover_usage :
+    forall (c : cumul) (t : task) (start sz : nat) (theta : asg),
+  eval_cumul c theta ->
+    Zle (eval_start t theta) (Z_of_nat start)
+    /\ Zlt (Z_of_nat (plus start sz)) (eval_end t theta) ->
+      task_usage t start sz theta = mult sz t.(resource).
+Proof.
+  intros; destruct H0 as [Hl Hu]; induction sz.
+    unfold task_usage; omega.
+    
+    unfold task_usage; fold task_usage. 
+    unfold task_at_time.
+
+Theorem task_bracket_usage :
+    forall (c : cumul) (t : task) (start : nat) (sz : nat) (theta : asg),
+  eval_cumul c theta ->
+    task_bracketed t start sz theta -> task_usage t start sz theta = mult t.(duration) t.(resource).
+Proof.
+  unfold task_bracketed, eval_start, eval_end; intros.
+  destruct H0 as [Hl Hu].
+  
+  induction sz.
+    unfold task_usage.
+    assert (le (duration t) 0).
+    apply (plus_le_reg_l (duration t) (0) (start)).
+    apply inj_le_iff.
+*)
 
 (* Check whether the ~cl -> [| s[t] >= lb |] /\ [| s[t]+d[t] < ub |]. *)
 
-
+(*
 Fixpoint span_area (ts : list task) (cl : clause) (lb ub : Z) :=
   match ts with
   | nil => 0%Z
@@ -47,7 +218,9 @@ Fixpoint span_area (ts : list task) (cl : clause) (lb ub : Z) :=
      if containedb t cl lb ub = true then 
        t.(resource)*t.(duration) + (span_area ts' cl lb ub)
      else
-       span_area ts' cl lb ub.
+       span_area ts' cl lb ub
+  end.
+*)
 
 Definition check_cumul (c : cumul) (cl : clause) : bool := false.
 
