checker/domain.v
@@ -3,18 +3,20 @@ Require Import ZArith.
 Require List.
 Require Import prim.
 Require Import bounds.
+Require Import zset.
 
 (* Exact representation of a variable domain. *)
 
 (* A bounded interval, and a set of gaps. *)
-Definition dom : Type := (dbound * (list Z))%type.
+Definition dom : Type := (dbound * zset)%type.
 
-Definition dom_unconstrained : dom := ((Unbounded, Unbounded), nil).
-Definition dom_const (k : Z) : dom := ((Bounded k, Bounded k), nil).
-Definition dom_neq (k : Z) : dom := ((Unbounded, Unbounded), cons k nil).
-Definition dom_le (k : Z) : dom := ((Unbounded, Bounded k), nil).
-Definition dom_ge (k : Z) : dom := ((Bounded k, Unbounded), nil).
+Definition dom_unconstrained : dom := ((Unbounded, Unbounded), empty).
+Definition dom_const (k : Z) : dom := ((Bounded k, Bounded k), empty).
+Definition dom_neq (k : Z) : dom := ((Unbounded, Unbounded), add empty k).
+Definition dom_le (k : Z) : dom := ((Unbounded, Bounded k), empty).
+Definition dom_ge (k : Z) : dom := ((Bounded k, Unbounded), empty).
 
+(*
 Fixpoint sat_holes (xs : list Z) (k : Z) := 
   match xs with
   | nil => True
@@ -24,7 +26,7 @@ Fixpoint sat_holes (xs : list Z) (k : Z) :=
 Fixpoint satb_holes (xs : list Z) (k : Z) :=
   match xs with
   | nil => true
-  | cons x xs' => negb (Z_eqb x k) && (satb_holes xs' k)
+  | cons x xs' => negb (Z_eqb x k) && negb (satb_holes xs' k)
   end.
 
 Theorem satb_holes_iff_holes : forall (ls : list Z) (k : Z),
@@ -56,14 +58,55 @@ Definition sat_dom (d : dom) (k : Z) :=
 
 Definition satb_dom (d : dom) (k : Z) :=
   satb_dbound (fst d) k && satb_holes (snd d) k.
+*)
+Definition sat_dom (d : dom) (k : Z) :=
+  sat_dbound (fst d) k /\ ~ mem (snd d) k.
+
+Definition satb_dom (d : dom) (k : Z) :=
+  satb_dbound (fst d) k && negb (memb (snd d) k).
 
 Theorem satb_dom_true_iff_dom : forall (d : dom) (k : Z),
   satb_dom d k = true <-> sat_dom d k.
 Proof.
   unfold satb_dom; unfold sat_dom. intros.
   rewrite andb_true_iff.
-  rewrite satb_dbound_iff_db; rewrite satb_holes_iff_holes.
-  tauto.
+  rewrite satb_dbound_iff_db.
+  rewrite negb_true_iff.
+  rewrite <- memb_true_iff_mem.
+  split.
+    intro; destruct H as [Hs Hm].
+    rewrite Hm.
+    split.
+      exact Hs.
+      apply diff_false_true.
+    
+    intro; destruct H as [Hs Hm].
+    split.
+      exact Hs.
+      apply not_true_is_false; exact Hm.
+Qed.
+
+Definition dom_meet (dx dy : dom) :=
+  (db_meet (fst dx) (fst dy), union (snd dx) (snd dy)).
+Theorem dom_meet_iff : forall (dx dy : dom) (k : Z),
+  sat_dom (dom_meet dx dy) k <-> sat_dom dx k /\ sat_dom dy k.
+Proof.
+  unfold sat_dom, dom_meet; intros.
+  destruct dx, dy; simpl.
+  rewrite mem_union_iff.
+  repeat (rewrite <- memb_true_iff_mem).
+  split.
+    intros; destruct H as [Hd Hm].
+    apply db_satmeet in Hd.
+    destruct Hd as [Hd Hd0].
+    split.
+      split. exact Hd. tauto.
+      split. exact Hd0. tauto.
+  
+    intro; destruct H as [Hl Hr].
+    destruct Hl as [Hd Hmd]; destruct Hr as [Hd0 Hmd0].
+    split.
+      apply db_sat_impl_meet. tauto. tauto.
 Qed.
 
 Definition dom_from_lit (x : ivar) (l : lit) :=
@@ -78,6 +121,7 @@ Definition dom_from_lit (x : ivar) (l : lit) :=
      if beq_nat x x' then dom_ge (k+1) else dom_unconstrained
   | _ => dom_unconstrained
   end.
+(*
 Theorem dom_from_lit_exact : forall (x : ivar) (l : lit) (theta : asg),
   eval_lit l theta <-> sat_dom (dom_from_lit x l) (eval_ivar x theta).
 Proof.
@@ -89,11 +133,71 @@ Proof.
   assert (beq_nat x i = true <-> x = i). apply beq_nat_true_iff.
   destruct beq_nat; simpl in *.
   assert (x = i). apply H; trivial.
-  rewrite <- H0. tauto.
+  rewrite <- H0. 
+  split.
+    intros.
+    eauto with zarith.
+    
+    intros.
+    destruct H1. destruct H1. exact H3.
+  
+  split.
+    intros.
+
 Qed.
+*)
 
 Fixpoint dom_from_negclause (x : ivar) (cl : clause) :=
   match cl with
   | nil => dom_unconstrained
-  | cons l : ls =>
-      dom_meet (dom_from_neglit l) (
+  | cons l ls =>
+      dom_meet (dom_from_lit x (neglit l)) (dom_from_negclause x ls)
+  end.
+(*
+Theorem dom_from_negclause_valid : forall (x : ivar) (cl : clause) (theta : asg),
+ ~eval_clause cl theta -> sat_dom (dom_from_negclause x cl) (eval_ivar x theta).
+Proof.
+  intros.
+  induction cl.
+  unfold dom_from_negclause, dom_unconstrained;
+  unfold sat_dom, sat_dbound; simpl. tauto.
+
+  unfold eval_clause in H; fold eval_clause in H.
+  unfold dom_from_negclause; fold dom_from_negclause.
+  assert (~(eval_lit a theta) /\ ~(eval_clause cl theta)).
+  apply Decidable.not_or; exact H. destruct H0.
+  assert (eval_lit (neglit a) theta).
+  apply neglit_not_lit. exact H0.
+  assert (sat_dom (dom_from_lit x (neglit a)) (eval_ivar x theta)).
+  apply dom_from_lit_valid; exact H2.
+  assert (sat_dbound (db_from_negclause x cl) (eval_ivar x theta)).
+  apply IHcl; exact H1.
+  apply db_sat_impl_meet. split. exact H3. exact H4.
+Qed.
+
+Theorem notdb_negclause_impl_clause : forall (x : ivar) (cl : clause) (theta : asg),
+  ~ sat_dbound (db_from_negclause x cl) (eval_ivar x theta) -> eval_clause cl theta.
+Proof.
+  intros.
+  assert (eval_clause cl theta \/ ~ eval_clause cl theta). apply dec_evalclause.
+  destruct H0.
+  
+  exact H0.
+  assert (sat_dbound (db_from_negclause x cl) (eval_ivar x theta)).
+  apply db_from_negclause_valid. exact H0.
+  tauto.
+Qed.
+
+Theorem notsat_ub_impl_notdb : forall (db : dbound) (k : Z),
+  ~ sat_ub (snd db) k -> ~ sat_dbound db k.
+Proof.
+  unfold sat_dbound; destruct db; simpl; intros.
+  tauto.
+Qed.
+
+Theorem notsat_lb_impl_notdb : forall (db : dbound) (k : Z),
+  ~ sat_lb (fst db) k -> ~ sat_dbound db k.
+Proof.
+  unfold sat_dbound; destruct db; simpl; intros. tauto.
+Qed.
+*)
