checker/element.v
@@ -1,7 +1,8 @@
 Require Import ZArith.
 Require Import Bool.
-Require Import prim.
 Require Import List.
+Require Import prim.
+Require Import bounds.
 
 (* Element constraint:
  * element x i [y_1, ..., y_n] <-> x = y_i.
@@ -15,7 +16,7 @@ Fixpoint eval_element_rec x i ys k theta :=
   match ys with
   | nil => False
   | cons y ys' =>
-    (eval_ivar i theta = k /\ eval_ivar x theta = eval_ivar y theta)
+    (eval_ivar i theta = k /\ eval_ivar x theta = y)
       \/ eval_element_rec x i ys' (k+1) theta
   end.
 
@@ -23,4 +24,29 @@ Definition eval_element (con : element) (theta : asg) :=
   match con with
   | Elem x i ys => eval_element_rec x i ys 0 theta
   end.
+
+Fixpoint check_element_rec x i ys k cl :=
+  match ys with
+  | nil => true
+  | cons y ys' =>
+    negb
+      (inbounds_negcl cl i k && inbounds_negcl cl x y)
+      && check_element_rec x i ys' (k+1) cl
+  end.
+Definition check_element elem cl :=
+  match elem with
+  | Elem x i ys => check_element_rec x i ys 0 cl
+  end.
+
+(*
+Theorem check_element_rec_valid :
+  forall (elt : element) (cl : clause),
+  check_element elt cl = true ->
+    implies (eval_element elt) (eval_clause cl).
+Proof.
+  unfold implies; destruct elt; intros.
+  induction l.
+Qed.
+   
+*)
 
