checker/zset.v
@@ -1,0 +1,130 @@
+(* Module for integer sets. *)
+Require Import Bool.
+Require Import ZArith.
+Require Import prim.
+
+Definition zset : Type := list Z.
+
+Definition empty : zset := nil.
+
+Fixpoint mem (s : zset) (k : Z) : Prop :=
+  match s with
+  | nil => False
+  | cons x xs => x = k \/ mem xs k
+  end.
+
+Fixpoint memb (s : zset) (k : Z) : bool :=
+  match s with
+  | nil => false
+  | cons x xs => (Z_eqb x k) || memb xs k
+  end.
+
+Theorem memb_true_iff_mem : forall (s : zset) (k : Z),
+  memb s k = true <-> mem s k.
+Proof.
+  intros. induction s.
+  unfold memb, mem.
+  split. intros; discriminate.
+  intros; tauto.
+
+  unfold memb, mem; fold memb; fold mem.
+  rewrite <- Z_eqb_iff_eq. rewrite <- IHs.
+  rewrite orb_true_iff. tauto.
+Qed.
+
+Definition add (s : zset) (k : Z) : zset :=
+  cons k s.
+Theorem mem_mem_add : forall (s : zset) (k : Z) (k' : Z),
+  mem s k -> mem (add s k') k.
+Proof.
+  intros; unfold add, mem. fold mem.
+  right. exact H.
+Qed.
+Theorem mem_k_addk : forall (s : zset) (k : Z),
+  mem (add s k) k.
+Proof.
+  intros; unfold add, mem; fold mem.
+  left. trivial.
+Qed.
+Theorem mem_addk_if : forall (s : zset) (k k' : Z),
+  mem (add s k) k' -> k = k' \/ mem s k'.
+Proof.
+  unfold add, mem; fold mem; intros.
+  exact H.
+Qed.
+
+Fixpoint rem (s : zset) (k : Z) :=
+  match s with
+  | nil => nil
+  | cons x xs =>
+    let tail := rem xs k in
+    if Z_eqb x k then tail else cons x tail
+  end.
+Theorem notmem_k_remk : forall (s : zset) (k : Z),
+  ~ mem (rem s k) k.
+Proof.
+  intros; induction s.
+
+  unfold mem, rem. tauto.
+
+  unfold rem; fold rem.
+  assert (Z_eqb a k = true <-> a = k). apply Z_eqb_iff_eq.
+  destruct (Z_eqb a k).
+
+  exact IHs.
+  unfold mem; fold mem.
+  rewrite <- memb_true_iff_mem in IHs.
+  rewrite <- memb_true_iff_mem.
+  rewrite <- H.
+  destruct (memb (rem s k) k).
+  tauto.
+  tauto.
+Qed.
+Theorem notmem_notmem_remk : forall (s : zset) (k k' : Z),
+  ~ mem s k' -> ~ mem (rem s k) k'.
+Proof.
+  intros s k k'; induction s.
+
+  unfold mem, rem; tauto.
+
+  unfold rem; fold rem. unfold mem; fold mem.
+  assert (Z_eqb a k = true <-> a = k). apply Z_eqb_iff_eq.
+  destruct (Z_eqb a k).
+  intros. apply IHs.
+  rewrite <- memb_true_iff_mem.
+  rewrite <- memb_true_iff_mem in H0.
+  destruct (memb s k').
+  tauto. tauto.
+
+  unfold mem; fold mem.
+  rewrite <- memb_true_iff_mem in IHs.
+  rewrite <- memb_true_iff_mem in IHs.
+  rewrite <- memb_true_iff_mem.
+  rewrite <- memb_true_iff_mem.
+  tauto.
+Qed.
+
+Fixpoint union (xs ys : zset) :=
+  match xs with
+  | nil => ys
+  | cons x xs' => add (union xs' ys) x
+  end.
+Theorem mem_union_iff : forall (xs ys : zset) (k : Z),
+  mem (union xs ys) k <-> mem xs k \/ mem ys k.
+Proof.
+  induction xs.
+    unfold union.
+    split.
+      intro. right. exact H.
+    
+      unfold mem; fold mem. tauto.
+
+    unfold union, mem; fold union; fold mem.
+    unfold add.
+    intros ys k.
+    assert (a = k \/ (mem xs k \/ mem ys k) <->
+      (a = k \/ mem xs k) \/ mem ys k). tauto.
+    rewrite <- H.
+    rewrite <- IHxs.
+    unfold mem; fold mem. tauto.
+Qed.
